examples/steel/arraystructs/FStar.PCM.POD.fsti
@@ -1,8 +1,7 @@
 module FStar.PCM.POD
 
 open FStar.PCM
-open FStar.PCM.Extras
-open AggregateRef
+open Steel.C.PCM
 open Steel.Effect
 
 let pod: Type u#a -> Type u#a = option
@@ -11,7 +10,7 @@ let none #a: Ghost.erased (pod a) = None
 
 let some (x: Ghost.erased 'a): Ghost.erased (pod 'a) = Some (Ghost.reveal x)
 
-let pod_pcm (a:Type): refined_one_pcm (pod a) = opt_pcm #a
+let pod_pcm (a:Type): pcm (pod a) = opt_pcm #a
 
 val pod_read
   (#a:Type) (#b:Type) (#x: Ghost.erased b)
